\documentclass{jsarticle}

\begin{document}

\begin{eqnarray*}
	P(\omega_{i} | X^{(n)}) &=& \frac{P(x_{n}|\omega_{i})}{\sum_{j=1}^{3}P(\omega_{j}|X^{(n-1)})P(x_{n}|\omega_{j})}\cdot P(\omega_{i}|X^{(n-1)}) & (i=1,2,3) \\
													&=& \frac{P(x_{n}|\omega_{i})}{P(\omega_{1}|X^{(n-1)})P(x_{n}|\omega_{1})+P(\omega_{2}|X^{(n-1)})P(x_{n}|\omega_{2})+P(\omega_{3}|X^{(n-1)})P(x_{n}|\omega_{3}) }\cdot P(\omega_{i}|X^{(n-1)}) \\ \\
	P(x_{n}|\omega_{i}) &=& \left\{
		\begin{array}{ll}
			\theta_{i} & (x_{n} = H) \\
			1 - \theta_{i} & (x_{n} = T) \\
		\end{array}
		\right
\end{eqnarray*}

\end{document}
